fix Addition

code/experimental/rsa/Addition.fst
@@ -9,41 +9,47 @@ module U32 = FStar.UInt32
 module U64 = FStar.UInt64
 
 type bignum = buffer FStar.UInt64.t
+type lbignum (len:U32.t) = 
+     b:bignum{length b = U32.v len} 
+
+type bnlen = (l:U32.t{U32.v l > 0 /\ U32.v l <= 8192})
 
 val sub_loop:
-    aLen:U32.t -> bLen:U32.t{U32.(bLen <=^ aLen)} ->
-    a:bignum{length a = U32.v aLen} -> b:bignum{length b = U32.v bLen} -> 
-    ind:U32.t{U32.(ind <=^ aLen)} -> carry:U64.t ->
-    res:bignum{length res = U32.v aLen} -> Stack unit
+    aLen:bnlen -> bLen:bnlen ->
+    a:lbignum aLen -> b:lbignum bLen{disjoint a b} ->
+    ind:U32.t{U32.v ind <= length a} -> carry:U64.t ->
+    res:lbignum aLen{disjoint res a /\ disjoint res b} -> Stack unit
     (requires (fun h -> live h a /\ live h b /\ live h res))
 	(ensures (fun h0 _ h1 -> live h0 a /\ live h0 b /\ live h0 res /\ 
         live h1 a /\ live h1 b /\ live h1 res /\ modifies_1 res h0 h1))
-let rec sub_loop aLen bLen a b ind carry res = 
-    let h0 = ST.get () in
+
+#set-options "--z3rlimit 150"
+
+let rec sub_loop aLen bLen a b ind carry res =
     if U32.(ind <^ aLen) then
         begin
         let t1 = a.(ind) in
-        let x =
-            if U32.(ind <^ bLen) then
-                (let t2 = b.(ind) in 
-                U64.(t1 -%^ t2))
-            else t1 in
-        res.(ind) <- U64.(x -%^ carry);
-        let carry = if U64.(x <^ carry) then 1uL else 0uL in
+        let t2 = if U32.(ind <^ bLen) then b.(ind) else 0uL in
+        res.(ind) <- U64.(t1 -%^ t2 -%^ carry);
+        let carry = 
+            (if U64.(carry =^ 1uL) then
+                (if U64.(t1 <=^ t2) then 1uL else 0uL)
+            else
+                (if U64.(t1 <^ t2) then 1uL else 0uL)) in
         let ind = U32.(ind +^ 1ul) in
         sub_loop aLen bLen a b ind carry res
         end
-    else ();
-    lemma_modifies_sub_1 h0 h0 res
 
 (* a must be greater than b *)
+(* ADD: isMore aLen bLen a b *)
 (* res = a - b *)
 val sub:
-    aLen:U32.t -> bLen:U32.t{U32.(bLen <=^ aLen)} ->
-    a:bignum{length a = U32.v aLen} -> b:bignum{length b = U32.v bLen} ->
-    res:bignum{length res = U32.v aLen} -> Stack unit
+    aLen:bnlen -> bLen:bnlen ->
+    a:lbignum aLen -> b:lbignum bLen{disjoint a b} ->
+    res:lbignum aLen{disjoint res a /\ disjoint res b} -> Stack unit
     (requires (fun h -> live h a /\ live h b /\ live h res))
 	(ensures (fun h0 _ h1 -> live h0 a /\ live h0 b /\  live h0 res /\
         live h1 a /\ live h1 b /\ live h1 res /\ modifies_1 res h0 h1))
+
 let sub aLen bLen a b res =
     sub_loop aLen bLen a b 0ul 0uL res
